\documentclass[11pt, oneside]{article} 
\usepackage{geometry}
\geometry{letterpaper} 
\usepackage{graphicx}
	
\usepackage{amssymb}
\usepackage{amsmath}
\usepackage{parskip}
\usepackage{color}
\usepackage{hyperref}

\graphicspath{{/Users/telliott/Github/precalculus/fig/}}
% \begin{center} \includegraphics [scale=0.4] {gauss3.png} \end{center}

\title{Parabola}
\date{}

\begin{document}
\maketitle
\Large

The parabola is one of a larger class of geometric figures called the conic sections.  
\begin{center} \includegraphics [scale=0.4] {conic_sections2.png} \end{center}

It is pretty complicated to look at parabolas in the way that the Greeks did, so we will fudge a little and use analytic geometry to get a general formula in Cartesian coordinates, so we can draw the curve.
\begin{center} \includegraphics [scale=0.35] {para_geo_1.png} \end{center}
The equation of a general parabola is simply $y=ax^2$, where $a$ is called the shape factor of the parabola.  

\begin{center} \includegraphics [scale=0.4] {shape_factor.png} \end{center}

The one in the figure is a little flatter than we usually draw, we'll see the reason for that choice in a minute.  At $x = 1$, $y = 1/4$, so $a = 1/4$.  Consistent with that, at $x = 2$ we have $y = ax^2 = 1$.

\subsection*{focus and directrix}

We need one more idea to start our geometric look at the parabola.  

The geometric definition is this.  Pick a point on the $y$-axis a distance $p$ up from the origin, colored magenta in the figure.  This point is called the focus ($F$).
\begin{center} \includegraphics [scale=0.35] {para_geo_1.png} \end{center}
Then draw a line parallel to the $x$-axis which intersects the $y$-axis the same distance $p$ below the origin.  This line is called the directrix.  It is colored blue and its equation is $y = -p$.

The parabola consists of all those points whose \emph{distance to the focus is equal to the vertical distance to the directrix}.

It is another fact that we will establish later that the distance $p$ is related to $a$ by the equation:
\[ 4ap = 1 \]
which explains our choice of $a$.  We need the parabola flat enough to see $F$ and the line $y = -p$ clearly.

If we consider the point $P = (2,1)$ we can compute the distance to the focus as simply $\Delta x = 2$ and to the directrix as $\Delta y = 1 + 1 = 2$.

\subsection*{slope of the tangent}

One last fact we will import from the future (to be justified in a bit).  At any point $(x,y)$ on the parabola, the slope is $2ax$.  Therefore, the slope of the tangent to the curve at $x = 2$ is 
\[ m = 2 \cdot 1/4 \cdot 2 = 1\]

By inspection of the graph we see that the tangent line goes through $I = (0,-1)$ which gives a point slope formula of $y = x -1$.  It is easy to verify that $(2,1)$ and $(0,-1)$ are both on the line, and of course the slope is $1$, as advertised.

Notice that the $x$-intercept, $x_0$ is
\[ 0 = x - 1, \ \ \ \ \ \ x = 1 \]
This is exactly halfway on the $x$-axis between $P$ and $I$.

\subsection*{another point}
From the equation of the curve we can get that $(x = \pm 1, y = 1/4)$ is on the curve, for either value of $x$.  The distance from each point to the directrix is just $1 \ 1/4$.
\begin{center} \includegraphics [scale=0.35] {para_geo_1.png} \end{center}

The distance to the focus is 
\[ \sqrt{1^2 + (\frac{3}{4})^2} = \sqrt{\frac{25}{16}} = \frac{5}{4} \]
which checks.

And this should not be a surprise.  A look at the figure will show that in units of $1/4$, we have a 3-4-5 right triangle.

\subsection*{computing p}

Pick an arbitrary point on a parabola (in blue), with coordinates $(x, ax^2)$.  The squared distance to the focus (magenta point) is 
\[ \Delta x^2 + \Delta y^2 =  x^2 + (ax^2 - p)^2  \]

while the squared distance to the directrix (red line) is  $(ax^2 + p)^2$ because $\Delta x$ is zero.  

\begin{center} \includegraphics [scale=0.4] {focus_dir.png} \end{center}

For the correct choice of $p$ these distances are to be equal:
\[ (ax^2 - p)^2 + x^2 = (ax^2 + p)^2 \]
\[ a^2 x^4 - 2ap x^2 + p^2 + x^2 = a^2x^4 + 2apx^2 + p^2 \]

Canceling two terms on each side
\[ - 2ap x^2 + x^2 =  + 2apx^2  \]
Divide by $x^2$
\[ - 2ap + 1 =  2ap  \]
\[ 4ap = 1 \]
\[ ap = \frac{1}{4} \]

The shape factor $a$ determines the distance of the focus from the origin, which is $p$, and from the directrix, which is $2p$.

\subsection*{slope of the tangent}
It will turn out that the slope of the tangent to $y=ax^2$ at any fixed point $x$ is equal to $2ax$. 

This is literally the first result from differential calculus, but we will also see a way to find it using analytical geometry, as well as a vector approach later on.

\begin{center} \includegraphics [scale=0.4] {para17.png} \end{center}

Thus, the equation of a line passing through the point $(x,ax^2)$ with the given slope is
\[ y' - ax^2 = 2ax(x' - x) \]
where $(x',y')$ is any other point on the line.

What \emph{that} means is that the $x$-intercept of the tangent line ($y' = 0$, $x' = x_0$) is:
\[ - ax^2 = 2ax x_0 - 2ax^2 \]
\[ ax^2 = 2ax x_0 \]
\[ x = 2x_0 \]
\[ x_0 = \frac{1}{2} x \]

The tangent line passes through the $x$ axis halfway back toward the origin.
\begin{center} \includegraphics [scale=0.4] {para17.png} \end{center}

And what \emph{that} means is that the $y$-intercept is symmetrical with the original point (as far below the $x$-axis as the point is above it). Here's the algebra:
\[ y_0 - ax^2 = 2ax(0 - x) \]
\[ y_0 = -ax^2 \]

And then finally, if the point on the parabola is $P$, the focus $F$, the intersection with the directrix $D$, and the $y$-intercept $I$

\begin{center} \includegraphics [scale=0.4] {para18.png} \end{center}
the quadrilateral $FPDI$ is a regular parallelogram with all four equal sides, and its long diagonal (the tangent line) makes equal angles with $FP$ and $PD$.

If $PD$ is extended vertically, the angle it makes with the tangent line is equal to the angle between $FP$ and the tangent line, so that for example, all vertical light rays entering a parabola will reflect and then come together at the focus.

\subsection*{analytic geometry}

A general formula for a parabola with its vertex at the point $(h,k)$ is
\[ y - k = a(x - h)^2 \]

where $a$ is called the \emph{shape factor}.  It governs how steeply the curve rises (and by its sign, in which direction it opens). Multiplying out:
\[ y - k = a(x^2 - 2xh + h^2) \]
\[ y = ax^2 - 2ah x + ah^2 + k \]

In this form the cofactors are usually simplified as
\[ y = ax^2 + bx + c \]

where
\[ b = -2ah; \ \ \ \ c = ah^2 + k \] 

This means that any parabola's shape is solely governed by the value of $a$.

If the equation is given in the second form then we can find:
\[ h = -\frac{b}{2a} \]
\[ k = c - ah^2 \]
\[ = c - \frac{b^2}{4a} \]

Probably the most common thing we're asked to do with a quadratic equation like this is to find the roots, the values of $x$ for which $y=0$ is a solution.  These are the points where the graph of the curve crosses the $x$-axis.

It is possible to have 0, 1 or 2 roots.  The black curve has two roots, the red curve has one.  The latter's equation is $y = x^2$, the former is $y = x^2 - 1$ and then we can see that $x^2 = 1$ has two real solutions $x = \pm 1$.

\begin{center} \includegraphics [scale=0.50] {para8.png} \end{center}

On the left, the magenta curve does not cross the $y$-axis.  Its equation is $y = x^2 + 1$, and there are no (real) solutions, no values of $x$ that solve the equation when $y = 0$.
\[ 0 = x^2 + 1 \]
\[ x^2 = - 1 \]

To find the roots of
\[ ax^2 + bx + c = 0 \]
We can guess solutions by trying to factor into a form like:
\[ (x - s)(x - t) = 0 \]

The case of a single root occurs when $s = t$ so we have $a(x - s)^2 = 0$.  A common example of that is a parabola with its vertex at the origin, so $s = 0$ and $y = ax^2$ (right panel, above).

Roots do not have to be integers (or even rational).  An arguably more productive and certainly more general approach to finding them is the process of \emph{completing the square}.  

First, multiply through by $1/a$ and rearrange:
\[ x^2 + \frac{b}{a} x = - \frac{c}{a} \]

The key insight is to recognize that if we add $(b/2a)^2$ to both sides, the left-hand side will become a perfect square:
\[ x^2 + \frac{b}{a} x + (\frac{b}{2a})^2 = -\frac{c}{a} + (\frac{b}{2a})^2 \]
\[ (x + \frac{b}{2a})^2 = -\frac{c}{a} + (\frac{b}{2a})^2 \]
\[ x + \frac{b}{2a} = \pm \sqrt{-\frac{c}{a} + (\frac{b}{2a})^2} \]

Multiplying top and bottom of the first term under the square root gives a common factor:
\[ x + \frac{b}{2a} = \pm \sqrt{-\frac{4ac}{4a^2} + (\frac{b}{2a})^2} \]
which can come out of the square root and then matches what's in the second term on the left-hand side:
\[ x + \frac{b}{2a} = \pm \frac{\sqrt{-4ac + b^2}}{2a} \]
which we rearrange slightly to give the standard \emph{quadratic formula}:
\[ x = \frac{-b \pm \sqrt{b^2 - 4ac}}{2a} \]


\subsection*{part 1}
Consider the simplest parabola:  $y = x^2$.

The point $(1,1)$ is on the curve, because $(x = 1, y = 1)$ satisfies the equation $y = x^2$.

\begin{center} \includegraphics [scale=0.50] {para11.png} \end{center}

Suppose we know that the slope of the tangent to the curve at the point $(1,1)$ is equal to $2$.

(Using calculus to find this result is trivial, we'll also show a non-calculus method in part three, below).  

The equation of the tangent line is
\[ y' - y = m(x' - x) \]
Plugging in for $(x', y') = (1,1)$:
\[ y - 1 = 2(x - 1) \]
\[ y = 2x - 1 \]

Now suppose that we knew only the parabola and this slope, but we did not know the point where the tangent meets the curve, and so do not know the $y$-intercept.

We have the equation of a line:
\[ y = 2x + y_0 \]

We seek points which are simultaneously on the line and the curve.  They must satisfy both equations.

Since this is a tangent line, we seek the value for which this expression has only a single solution.  The tangent "touches" the curve at a single point.

So, substitute for $y$ from the equation for the curve:
\[ x^2 = 2x + y_0 \]
\[ x^2 - 2x - y_0 = 0 \]

Now look at the quadratic formula we would use to solve this equation for $x$:
\[ x = \frac{-b \pm \sqrt{b^2 - 4ac}}{2a} \]

There is a single solution when the part under the square root (called the discriminant) is equal to zero.

\[ b^2 - 4ac = 0 \]
\[ b^2 = 4ac \]
\[ (-2)^2 = 4(-y_0) \]
\[ y_0 = -1 \]
Therefore, the equation of the tangent line is $y = 2x - 1$, which matches what we had before.

In general, $y = 2x + y_0$ is a \emph{family} of lines.  For $y_0 = -1$, there is a single solution for $x$ to be both on the line and the parabola.  For $y_0 < -1$, there are no solutions, while for $y_0 > -1$ there are two solutions, because the line actually traces out a secant of the parabola, passing through the curve at two points.

\subsection*{part 2}
Now suppose we have the same parabola and a point not on the parabola, but in the plane and outside of the "cup" of the parabola, such as $(3,5)$.  We seek the equations of tangent lines to the parabola that go through this point.  
\begin{center} \includegraphics [scale=0.4] {para12.png} \end{center}

There will be two of them.  We show just one in the figure.

The equations of lines passing through this point, with different slopes $m$ are given by:

\[ (y' - y) = m(x' - x) \]
Here, let $(x',y')$ be $(3,5)$ and then multiply by $-1$:

\[ 5 - y = m(3 - x) \]
\[ y - 5 = m(x - 3) \]

Since values of $(x,y)$ are both on the line and the parabola $y=x^2$, we can plug in for $y$:
\[ x^2 - 5 = mx - 3m \]
\[ x^2 - mx + (3m - 5) = 0 \]

As before, solutions are given by the quadratic equation.  The value of the slope $m$ giving a single solution (zero discriminant) is:
\[ (-m)^2 - 4(3m - 5) = 0 \]
\[ m^2 - 12m + 20 = 0 \]
\[ (m - 2)(m - 10) = 0 \]
\[ m = 2, \ \ \ m = 10 \]

We knew the first one already, because the point $(3,5)$ is on the line $y = 2x - 1$.  This is the tangent to the curve at $(1,1)$, which has slope $m = 2$.
\begin{center} \includegraphics [scale=0.50] {para13.png} \end{center}

Actually, there is always another solution which we haven't found explicitly and isn't shown on the graph either.  Any vertical line (with infinite slope) passes through only a single point on the parabola.

Basically what this amounts to is that in the equation
\[ x = \frac{m \pm \sqrt{(-m)^2 - 4(3m - 5)}}{2} \]

as $m$ gets very large, only the term $(-m)^2$ matters under the square root, so we have
\[ x = \frac{m \pm \sqrt{(-m)^2}}{2} \]
if we choose the negative root, then as $m \rightarrow \infty$, $m - \sqrt{m^2} \rightarrow 0$.

\subsection*{part 3}
Now suppose we are given the same parabola again and also a point on it such as $(x_1,y_1)$.  

Any line through that point has the equation:
\[ y - y' = m(x - x') \]

To find the equation of a tangent line through that point we need the slope $m$.

If there is a point $(x,y)$ that is on the line and \emph{also} on the parabola, it must satisfy $y = ax^2$ as well, so:
\[ ax^2 - ax'^2 = m(x - x') \]
\[ ax^2 - mx - ax'^2 + mx' = 0 \]

Certainly $x = x'$ is a solution.

The value of $m$ must be such that there are \emph{no other solutions}.

Write the quadratic equation to solve for $x$:
\[ x = \frac{m \pm \sqrt{m^2 - 4a(mx' - ax'^2)}}{2a} \]

There is a single solution when the discriminant is zero, that is, when
\[ x = \frac{m}{2a} \]
\[ m = 2ax \]

Since $x = x'$ for the tangent line
\[ m = 2ax' \]
as expected.

The slope of the tangent line is $2ax'$ and in particular, at the point $(1,1)$, the slope is equal to $2$.

\subsection*{further comment}

The slope of the parabola has some simple interesting properties.  For example, pick any two points $(x,y)$ and $(x',y')$ on our standard parabola.

The slope of the line that connects those two points is equal to the slope of the parabola at the point whose $x$-value is halfway in between.  
\begin{center} \includegraphics [scale=0.4] {para19.png} \end{center}

For the first part:
\[ m = \frac{y'-y}{x'-x} \]
\[ = \frac{ax'^2 - ax^2}{x'-x} \]
\[ = a \ [ \ \frac{x'^2 - x^2}{x' - x} \ ] \]
\[ = a(x' + x) \]

For the midpoint
\[ x_m = \frac{1}{2} (x' + x) \]
and the slope is
\[ 2a \cdot \frac{1}{2} (x' + x) \]
\[ = a(x' + x) \]

A similar result is that if we pick any two points $(x,y)$ and $(x',y')$, and draw their slopes, the point where the two slope lines meet has its $x$-value exactly halfway in between $x$ and $x'$.

\end{document}